Challenge/Bls12381/ProofSupport.lean
@@ -20,6 +20,7 @@ import Challenge.Bls12381.ProofSupport.LawfulFp2
 import Challenge.Bls12381.ProofSupport.Fp2
 import Challenge.Bls12381.ProofSupport.Fp2Representation
 import Challenge.Bls12381.ProofSupport.Fp2SourceDefs
+import Challenge.Bls12381.ProofSupport.Fp2SourceSchedule
 import Challenge.Bls12381.ProofSupport.Fp2Source
 import Challenge.Bls12381.ProofSupport.Fp2SourceLawful
 import Challenge.Bls12381.ProofSupport.LawfulFp6
